

①

$$a) \text{ mean} = \sum_k \pi_k \mu_k$$

$$\text{cov} = \sum_k \pi_k \Sigma_k$$

②

$$a) P(f(x) \neq y) \geq \frac{H(Y|X) - 1}{\log(|Y|)}$$

$$b) \text{ MAP: } \hat{y} = \underset{y}{\operatorname{argmax}} P(x|y) P(y)$$

$$P(y = \text{fish}) = \frac{3}{8} \quad P(y = \text{cat}) = \frac{1}{4} \quad P(y = \text{dog}) = \frac{3}{8}$$

$P(x y) P(y)$	$y = \text{fish}$	cat	dog
$x=1$	$\frac{3}{32}$	$\frac{1}{32}$	$\frac{3}{8 \cdot 16}$
2	$\frac{3}{32 \cdot 16}$	0	$\frac{3}{32}$
3	0	$\frac{1}{32}$	$\frac{3}{8 \cdot 16}$
4	$\frac{1}{32 \cdot 16}$	0	0

 \Rightarrow

	\hat{y}
$x=1$	fish
2	dog
3	cat
4	fish

	error rate
$x=1$	$\frac{1}{8} + \frac{1}{16}$
2	$\frac{1}{16}$
3	$\frac{1}{16}$
4	0

$$\text{error rate} = \frac{3+2}{16} = \frac{5}{16}$$

$$\begin{aligned}
 c) \quad H(E, Y | \hat{Y}) &= H(E | \hat{Y}) + H(Y | E, \hat{Y}) \\
 &\leq H(E) + H(Y | E, \hat{Y}) \\
 &= (1 - p_e) \log_2 \left(\frac{1}{1 - p_e} \right) + p_e \log_2 \left(\frac{1}{p_e} \right) + H(Y, E, \hat{Y}) \\
 &= (1 - p_e) \log_2 \left(\frac{1}{1 - p_e} \right) + p_e \log_2 \left(\frac{1}{p_e} \right) + p_e \log_2 |Y|.
 \end{aligned}$$

While $H(E, Y | \hat{Y}) \geq H(Y | X)$, we have:

$$\begin{aligned}
 H(Y | X) &\leq (1 - p_e) \log_2 \left(\frac{1}{1 - p_e} \right) + p_e \left(\log_2 \left(\frac{1}{p_e} \right) + \log_2 |Y| \right) \\
 &= p_e \left(\log_2 \left(\frac{1}{p_e} \right) + \log_2 |Y| - \log_2 \left(\frac{1}{1 - p_e} \right) \right) + \log_2 \left(\frac{1}{1 - p_e} \right) \\
 \therefore p_e &\geq \frac{H(Y | X) - \log_2 \left(\frac{1}{1 - p_e} \right)}{\log_2 \left(\frac{1}{p_e} \right) + \log_2 |Y| - \log_2 \left(\frac{1}{1 - p_e} \right)}
 \end{aligned}$$